Eliminate redundant or duplicated list material from HOL Light core
This avoids the use of the local function LIST_OF_FUN in favour of
the equivalent (modulo argument order) from the core, list_of_seq.
Moreover the conversions LIST_OF_SEQ_CONV, LENGTH_CONV and EL_CONV,
which are set up in the HOL Light core as of this commit

  https://github.com/jrh13/hol-light/commit/c0953a80cde3f07677c2f5e5404be08862aec9b5

are used in place of s2n-bignum versions.

common/misc.ml
@@ -18,25 +18,13 @@ needs "Library/words.ml";;
 (* Additional list lemmas, operations and conversions.                       *)
 (* ------------------------------------------------------------------------- *)
 
-let LENGTH_FILTER = prove
- (`!P l:A list. LENGTH(FILTER P l) <= LENGTH l`,
-  GEN_TAC THEN LIST_INDUCT_TAC THEN ASM_REWRITE_TAC[FILTER; LE_REFL] THEN
-  COND_CASES_TAC THEN REWRITE_TAC[LENGTH] THEN ASM_ARITH_TAC);;
-
-let LIST_OF_FUN = define
- `LIST_OF_FUN 0 (f:num->A) = [] /\
-  LIST_OF_FUN (SUC n) f = APPEND (LIST_OF_FUN n f) [f n]`;;
-
-let LIST_OF_FUN_CLAUSES = prove
- (`(!(f:num->A). LIST_OF_FUN 0 f = []) /\
-   (!(f:num->A). LIST_OF_FUN 1 f = [f 0]) /\
-   (!(f:num->A). LIST_OF_FUN 2 f = [f 0; f 1]) /\
-   (!(f:num->A). LIST_OF_FUN 3 f = [f 0; f 1; f 2]) /\
-   (!(f:num->A). LIST_OF_FUN 4 f = [f 0; f 1; f 2; f 3])`,
-  REPEAT STRIP_TAC THEN
-  CONV_TAC(LAND_CONV(TOP_DEPTH_CONV num_CONV)) THEN
-  REWRITE_TAC[LIST_OF_FUN; APPEND] THEN
-  CONV_TAC NUM_REDUCE_CONV);;
+let LIST_OF_SEQ_CLAUSES = prove
+ (`(!(f:num->A). list_of_seq f 0 = []) /\
+   (!(f:num->A). list_of_seq f 1 = [f 0]) /\
+   (!(f:num->A). list_of_seq f 2 = [f 0; f 1]) /\
+   (!(f:num->A). list_of_seq f 3 = [f 0; f 1; f 2]) /\
+   (!(f:num->A). list_of_seq f 4 = [f 0; f 1; f 2; f 3])`,
+  CONV_TAC(ONCE_DEPTH_CONV LIST_OF_SEQ_CONV) THEN REWRITE_TAC[]);;
 
 let SUB_LIST = define
  `SUB_LIST (0,0) l = [] /\
@@ -155,21 +143,6 @@ let SUB_LIST_APPEND_LEFT = prove
 
 let TRIM_LIST = define
  `TRIM_LIST (h,t) l = SUB_LIST (h,LENGTH l - (h + t)) l`;;
-
-let EL_CONV =
-  let conv0 = GEN_REWRITE_CONV I [CONJUNCT1 EL] THENC GEN_REWRITE_CONV I [HD]
-  and conv1 = GEN_REWRITE_CONV I [CONJUNCT2 EL]
-  and convt = GEN_REWRITE_CONV I [TL] in
-  let convs = LAND_CONV num_CONV THENC conv1 THENC RAND_CONV convt in
-  let rec conv tm = (conv0 ORELSEC (convs THENC conv)) tm in
-  conv;;
-
-let rec LENGTH_CONV =
-  let conv0 = GEN_REWRITE_CONV I [CONJUNCT1 LENGTH]
-  and conv1 = GEN_REWRITE_CONV I [CONJUNCT2 LENGTH] in
-  let rec conv tm =
-   (conv0 ORELSEC (conv1 THENC RAND_CONV conv THENC NUM_SUC_CONV)) tm in
-  conv;;
 
 let SUB_LIST_CONV =
   let [cth1;cth2;cth3;cth4] = CONJUNCTS SUB_LIST_CLAUSES in
@@ -1452,7 +1425,7 @@ let word_subdeinterleave = define
 
 let word_deinterleave = define
  `(word_deinterleave:num->num->M word->(N word)list) l n z =
-    LIST_OF_FUN l (word_subdeinterleave l n z)`;;
+    list_of_seq (word_subdeinterleave l n z) l`;;
 
 let WORD_DEINTERLEAVE_CLAUSES = prove
  (`(word_deinterleave:num->num->M word->(N word)list) 2 n z =
@@ -1461,7 +1434,7 @@ let WORD_DEINTERLEAVE_CLAUSES = prove
    [word_subdeinterleave 3 n z 0;
     word_subdeinterleave 3 n z 1;
     word_subdeinterleave 3 n z 2]`,
-  REWRITE_TAC[word_deinterleave; LIST_OF_FUN_CLAUSES]);;
+  REWRITE_TAC[word_deinterleave; LIST_OF_SEQ_CLAUSES]);;
 
 (* ------------------------------------------------------------------------- *)
 (* Conversion for word_subdeinterleave and word_interleave. These are very   *)
